Interfaces and private keyword for FlexTLS.Record.fst

src/flex/FlexTLS.Record.fst
@@ -3,11 +3,13 @@
 module FlexTLS.Record
 
 
-open Log
+open Platform
+open Platform.Log
 open Platform.Tcp
 open Platform.Bytes
 open Platform.Error
 
+open MiTLS
 open MiTLS.TLSInfo
 open MiTLS.TLSConstants
 
@@ -21,22 +23,24 @@ open FlexTLS.State
 let log = Log.retrieve "FlexTLS.Log.General"
 
 /// <summary>
-/// Get fragment size depending on the fragmentation policy
+/// PRIVATE : Get fragment size depending on the fragmentation policy
 /// </summary>
 /// <param name="fp"> Fragmentation policy </param>
 /// <returns> size of the fragment to be applied </returns>
-let fs_of_fp (fp:fragmentationPolicy) : int =
+private val fs_of_fp : (fp:fragmentationPolicy) -> int 
+let fs_of_fp fp =
   match fp with
-  | All(n) | One(n) -> n
+  | All n | One n -> n
 
 /// <summary>
-/// Split any payload depending on the fragmentation size
+/// PRIVATE : Split any payload depending on the fragmentation size
 /// </summary>
 /// <param name="bytes"> Data bytes to be split </param>
 /// <param name="fp"> Fragmentation policy </param>
 /// <returns> Fragment of the chosen size * remaining unsplit data bytes </returns>
 // BB FIXME This function uses the .NET Framework
-let splitPayloadFP (b:bytes) (fp:fragmentationPolicy) : bytes * bytes =
+private val splitPayloadFP : (b:bytes) -> (fp:fragmentationPolicy) -> bytes * bytes
+let splitPayloadFP b fp =
   let len = System.Math.Min((length b),(fs_of_fp fp)) in
   Bytes.split b len
 
@@ -46,21 +50,21 @@ let splitPayloadFP (b:bytes) (fp:fragmentationPolicy) : bytes * bytes =
 /// <param name="channel"> Channel to extract buffer from </param>
 /// <param name="ct"> Content type </param>
 /// <returns> Buffer associated to the chosen content type </returns>
-let pickCTBuffer (ch:channel) (ct:ContentType) : bytes =
+private val pickCTBuffer : (ch:channel) -> (ct:ContentType) -> bytes
+let pickCTBuffer ch ct =
   match ct with
   | Handshake         -> ch.hs_buffer
   | Alert             -> ch.alert_buffer
   | Application_data  -> ch.appdata_buffer
   | _ -> failwith "Unsupported content type"
 
-
-
 /// <summary>
-/// Read a record fragment header to get ContentType, ProtocolVersion and Length of the fragment
+/// PRIVATE : Read a record fragment header to get ContentType, ProtocolVersion and Length of the fragment
 /// </summary>
 /// <param name="st"> State of the current Handshake </param>
 /// <returns> ContentType * ProtocolVersion * Length * Header bytes </returns>
-let parseFragmentHeader (st:state) : ContentType * ProtocolVersion * nat * bytes =
+private val parseFragmentHeader : (st:state) -> ContentType * ProtocolVersion * nat * bytes
+let parseFragmentHeader st =
   match Tcp.read st.ns 5 with
   | Error x -> failwith (perror __SOURCE_FILE__ __LINE__ x)
   | Correct header ->
@@ -69,24 +73,25 @@ let parseFragmentHeader (st:state) : ContentType * ProtocolVersion * nat * bytes
     | Correct(ct,pv,len) -> ct,pv,len,header
 
 /// <summary>
-/// Get N bytes from the network stream and decrypts it as a fragment
+/// PRIVATE : Get N bytes from the network stream and decrypts it as a fragment
 /// </summary>
 /// <param name="st"> State of the current Handshake </param>
 /// <param name="ct"> Content type of the fragment </param>
 /// <param name="len"> Length of the fragment </param>
 /// <returns> Updated state (reading side) * decrypted plaintext </returns>
-let getFragmentContent (st:state) (ct:ContentType) (len:int) : state * bytes =
+private val getFragmentContent : (st:state) -> (ct:ContentType) -> (len:int) -> state * bytes =
+let getFragmentContent st ct len =
   match Tcp.read st.ns len with
   | Error x -> failwith (perror __SOURCE_FILE__ __LINE__ x)
   | Correct payload ->
     match Record.recordPacketIn st.read.epoch st.read.record ct payload with
     | Error (ad,x) -> failwith (perror __SOURCE_FILE__ __LINE__ x)
     | Correct (rec_in,rg,frag)  ->
-      let st = FlexState.updateIncomingRecord st rec_in in
+      let st = State.updateIncomingRecord st rec_in in
       let id = TLSInfo.mk_id st.read.epoch in
       let fragb = TLSFragment.reprFragment id ct rg frag in
-      let st = FlexState.updateLog st ct fragb in
-      Log.logTrace(sprintf "+++ Record : %s" (Bytes.hexString fragb));
+      let st = State.updateLog st ct fragb in
+      Log.write log Trace "Record Payload" (sprintf "+++ Record : %s" (Bytes.hexString fragb));
       (st,fragb)
 
 /// <summary>
@@ -94,9 +99,10 @@ let getFragmentContent (st:state) (ct:ContentType) (len:int) : state * bytes =
 /// </summary>
 /// <param name="st"> State of the current Handshake </param>
 /// <returns> State * ContentType * ProtocolVersion * Lenght of the record payload * Fragment header bytes * Fragment payload bytes </returns>
-let receive (st:state) : state * ContentType * ProtocolVersion * int * bytes * bytes =
-  let ct,pv,len,header = FlexRecord.parseFragmentHeader st in
-  let st,payload = FlexRecord.getFragmentContent st ct len in
+val receive : (st:state) -> state * ContentType * ProtocolVersion * int * bytes * bytes =
+let receive st =
+  let ct,pv,len,header = parseFragmentHeader st in
+  let st,payload = getFragmentContent st ct len in
   st,ct,pv,len,header,payload
 
 /// <summary>
@@ -108,11 +114,12 @@ let receive (st:state) : state * ContentType * ProtocolVersion * int * bytes * b
 /// <param name="ct"> Content type of the fragment </param>
 /// <param name="payload"> Data to encrypt </param>
 /// <returns> Updated incoming record state * ciphertext </returns>
-let encrypt (e:epoch) (pv:ProtocolVersion) (k:Record.ConnectionState) (ct:ContentType) (payload:bytes) : Record.ConnectionState * bytes =
+private val encrypt : (e:epoch) -> (pv:ProtocolVersion) -> (k:Record.ConnectionState) -> (ct:ContentType) -> (payload:bytes) -> Record.ConnectionState * bytes
+let encrypt e pv k ct payload =
 // pv is the protocol version set in the record header.
 // For encrypting epochs, it'd better match the protocol version contained in the epoch, since the latter is used for the additional data
   let len = length payload in
-  let rg : Range.range = (len,len) in
+  let rg = (len,len) in
   let id = TLSInfo.mk_id e in
   let frag = TLSFragment.fragment id ct rg payload in
   let k,b = Record.recordPacketOut e k pv rg ct frag in
@@ -125,12 +132,13 @@ let encrypt (e:epoch) (pv:ProtocolVersion) (k:Record.ConnectionState) (ct:Conten
 /// <param name="stout"> State of the current Handshake on the outgoing side </param>
 /// <param name="fp"> Optional fragmentation policy applied to the message </param>
 /// <returns> Updated incoming state * Updated outgoing state * forwarded record bytes </returns>
-let forward (stin:state) (stout:state) (*?*)(fp:fragmentationPolicy) : state * state * bytes =
+val forward : (stin:state) -> (stout:state) -> (*?*)(fp:fragmentationPolicy) -> state * state * bytes
+let forward stin stout fp =
   //  let fp = defaultArg fp FlexConstants.defaultFragmentationPolicy in
-  let ct,pv,len,header = FlexRecord.parseFragmentHeader stin in
-  let stin,payload = FlexRecord.getFragmentContent stin ct len in
-  let stout = FlexState.updateOutgoingBuffer stout ct payload in
-  let stout = FlexRecord.send stout ct fp in
+  let ct,pv,len,header = parseFragmentHeader stin in
+  let stin,payload = getFragmentContent stin ct len in
+  let stout = State.updateOutgoingBuffer stout ct payload in
+  let stout = send stout ct fp in
   stin,stout,payload
 
 /// <summary>
@@ -141,13 +149,14 @@ let forward (stin:state) (stout:state) (*?*)(fp:fragmentationPolicy) : state * s
 /// <param name="fp"> Optional fragmentation policy applied to the message </param>
 /// <returns> Updated outgoing record state </returns>
 /// <remarks> We leave the remainder in the buffer </remarks>
-let send (st:state) (ct:ContentType) (*?*)(fp:fragmentationPolicy) : state =
+val send : (st:state) -> (ct:ContentType) -> (*?*)(fp:fragmentationPolicy) -> state =
+let rec send st ct fp =
   //  let fp = defaultArg fp FlexConstants.defaultFragmentationPolicy in
   let payload = pickCTBuffer st.write ct in
-  let k,b,rem = FlexRecord.send st.ns st.write.epoch st.write.record ct payload st.write.epoch_init_pv fp in
-  let st = FlexState.updateLog st ct b in
-  let st = FlexState.updateOutgoingBuffer st ct rem in
-  let st = FlexState.updateOutgoingRecord st k in
+  let k,b,rem = send st.ns st.write.epoch st.write.record ct payload st.write.epoch_init_pv fp in
+  let st = State.updateLog st ct b in
+  let st = State.updateOutgoingBuffer st ct rem in
+  let st = State.updateOutgoingRecord st k in
   st
 
 /// <summary>
@@ -161,7 +170,8 @@ let send (st:state) (ct:ContentType) (*?*)(fp:fragmentationPolicy) : state =
 /// <param name="epoch_init_pv"> Optional Protocol version set for the Initial epoch </param>
 /// <param name="fp"> Optional fragmentation policy applied to the message </param>
 /// <returns> Updated outgoing record state * remainder of the plain data </returns>
-let send (ns:NetworkStream) (e:epoch) (k:Record.ConnectionState) (ct:ContentType) (payload:bytes) (*?*)(epoch_init_pv:ProtocolVersion) (*?*)(fp:fragmentationPolicy) : Record.ConnectionState * bytes * bytes =
+val send_2 : (ns:NetworkStream) -> (e:epoch) -> (k:Record.ConnectionState) -> (ct:ContentType) -> (payload:bytes) -> (*?*)(epoch_init_pv:ProtocolVersion) -> (*?*)(fp:fragmentationPolicy) -> Record.ConnectionState * bytes * bytes
+let rec send_2 ns e k ct payload epoch_init_pv fp =
   //  let fp = defaultArg fp FlexConstants.defaultFragmentationPolicy in
   let pv =
   if TLSInfo.isInitEpoch e then
@@ -174,14 +184,14 @@ let send (ns:NetworkStream) (e:epoch) (k:Record.ConnectionState) (ct:ContentType
   in
   let msgb,rem = splitPayloadFP payload fp in
   Log.write log Trace "Record Payload" (sprintf "+++ Record : %s" (Bytes.hexString msgb));
-  let k,b = FlexRecord.encrypt e pv k ct msgb in
+  let k,b = encrypt e pv k ct msgb in
   match Tcp.write ns b with
   | Error x -> failwith x
   | Correct() ->
     match fp with
     | All(fs) ->
       if rem = empty_bytes then (k,msgb,rem) else
-        let k,b,rem = FlexRecord.send ns e k ct rem pv fp in k,(msgb @| b),rem
+        let k,b,rem = send_2 ns e k ct rem pv fp in k,(msgb @| b),rem
     | One(fs) -> (k,msgb,rem)
 
 /// <summary>
@@ -193,7 +203,8 @@ let send (ns:NetworkStream) (e:epoch) (k:Record.ConnectionState) (ct:ContentType
 /// <param name="payload"> Data to encrypt </param>
 /// <param name="fp"> Optional fragmentation policy applied to the message </param>
 /// <returns> Remaining bytes </returns>
-let send_raw (ns:NetworkStream) (ct:ContentType) (pv:ProtocolVersion) (payload:bytes) (*?*)(fp:fragmentationPolicy) : bytes =
+val send_raw : (ns:NetworkStream) -> (ct:ContentType) -> (pv:ProtocolVersion) -> (payload:bytes) -> (*?*)(fp:fragmentationPolicy) -> bytes
+let rec send_raw ns ct pv payload fp =
   //  let fp = defaultArg fp FlexConstants.defaultFragmentationPolicy in
   let b,rem = splitPayloadFP payload fp in
   let fragb = Record.makePacket ct pv b in
@@ -203,5 +214,5 @@ let send_raw (ns:NetworkStream) (ct:ContentType) (pv:ProtocolVersion) (payload:b
   | Correct() ->
     match fp with
     | All(fs) ->
-      if rem = empty_bytes then empty_bytes else FlexRecord.send_raw ns ct pv rem fp
+      if rem = empty_bytes then empty_bytes else send_raw ns ct pv rem fp
     | One(fs) -> rem
